extracted signal map

fairness/lawyer/examples/eo_fin/eo_fin.v
@@ -5,7 +5,7 @@ From trillium.fairness Require Import locales_helpers utils.
 From trillium.fairness.lawyer Require Import program_logic sub_action_em.
 From trillium.fairness.lawyer.obligations Require Import obligations_model obls_utils obligations_resources obligations_logic obligations_em.
 From trillium.fairness.heap_lang Require Export heap_lang_defs tactics notation sswp_logic locales_helpers_hl.
-From trillium.fairness.lawyer.examples Require Import bounded_nat.
+From trillium.fairness.lawyer.examples Require Import bounded_nat signal_map.
 
 
 Close Scope Z.
@@ -13,348 +13,6 @@ Close Scope Z.
 Definition EODegree n := bounded_nat n. 
 Definition EOLevel n := bounded_nat n.
 
-
-Section SignalMap.
-
-  Class SigMapPreG Σ := {
-      sm_sig_map :> inG Σ (authUR (gmapUR nat (agreeR SignalId)));
-  }.
-  
-  Class SigMapG Σ := {
-      sm_PreG :> SigMapPreG Σ;
-      sm_γ__smap: gname;
-  }.
-
-  Context `{SigMapG Σ}.
-
-  Context `{DISCR__d: OfeDiscrete DegO} `{DISCR__l: OfeDiscrete LevelO}.
-  Context {LEQUIV__l: @LeibnizEquiv (ofe_car LevelO) (ofe_equiv LevelO)}.   
-  Let Degree := ofe_car DegO.
-  Let Level := ofe_car LevelO.
-  (* Context `{OP: ObligationsParams Degree Level Locale LIM_STEPS}. *)
-  Context `{OP': ObligationsParamsPre Degree Level LIM_STEPS}.
-  Let EO_OP := LocaleOP (Locale := locale heap_lang). 
-  Existing Instance EO_OP. 
-
-  Context {oGS: ObligationsGS Σ}.
-
-  Context (L: nat -> Level). 
-
-  Definition ex_ith_sig B (i: nat) (s: SignalId): iProp Σ :=
-    sgn s (L i) (Some $ B i) (oGS := oGS). 
-  
-  Definition smap_repr B K (smap: gmap nat SignalId): iProp Σ :=
-    own sm_γ__smap (● (to_agree <$> smap: gmapUR nat (agreeR SignalId))) ∗
-    ⌜ dom smap = set_seq 0 K ⌝ ∗
-    ([∗ map] i ↦ s ∈ smap, ex_ith_sig B i s).
-
-  Definition ith_sig (i: nat) (s: SignalId): iProp Σ :=
-    own sm_γ__smap (◯ {[ i := to_agree s ]}).
-
-  Lemma ith_sig_in i s B K (smap: gmap nat SignalId):
-    ⊢ ith_sig i s -∗ smap_repr B K smap -∗ ⌜ smap !! i = Some s ⌝.
-  Proof using.
-    iIntros "S (SM & ? & ?)". iCombine "SM S" as "SM".
-    iDestruct (own_valid with "SM") as %V.
-    apply auth_both_valid_discrete in V as [V ?].
-    apply singleton_included_l in V. destruct V as (x & ITH & LE).
-    iPureIntro.
-    rewrite Some_included_total in LE.
-    destruct (to_agree_uninj x) as [y X].
-    { eapply lookup_valid_Some; eauto. done. }
-    rewrite -X in LE. apply to_agree_included in LE.
-    rewrite -X in ITH.
-    
-    eapply leibniz_equiv.       
-    rewrite lookup_fmap in ITH.
-    rewrite -LE in ITH.
-    
-    apply fmap_Some_equiv in ITH as (?&ITH&EQ).
-    rewrite ITH. apply to_agree_inj in EQ. by rewrite EQ.
-  Qed.
-
-  Lemma ith_sig_sgn i s B K (smap: gmap nat SignalId):
-    ⊢ ith_sig i s -∗ smap_repr B K smap -∗ sgn s (L i) None (oGS := oGS).
-  Proof using.
-    iIntros "S SR".
-    iDestruct (ith_sig_in with "[$] [$]") as "%ITH". 
-    iDestruct "SR" as "(SM & % & ?)".
-    iDestruct (big_sepM_lookup with "[$]") as "ITH"; eauto.
-    rewrite /ex_ith_sig.     
-    by iDestruct (sgn_get_ex with "[$]") as "[??]". 
-  Qed.
-
-  Lemma smap_repr_split B K smap i s:
-    ⊢ ith_sig i s -∗ smap_repr B K smap -∗
-      ex_ith_sig B i s ∗ (ex_ith_sig B i s -∗ smap_repr B K smap).
-  Proof using.
-    iIntros "#ITH SR".
-    iDestruct (ith_sig_in with "[$] [$]") as "%ITH".
-    rewrite /smap_repr. iDestruct "SR" as "(SM & % & SR)".
-    rewrite {2 5}(map_split smap i) ITH /=.
-    rewrite !big_sepM_union.
-    2: apply map_disjoint_singleton_l_2; by apply lookup_delete.
-    iDestruct "SR" as "[S SR]". rewrite big_sepM_singleton.
-    iFrame. iIntros. iFrame. done.
-  Qed.
-
-  Lemma smap_repr_split_upd B B' m smap i s
-    (OTHER_PRES: forall j, j ≠ i -> j ∈ dom smap -> B' j = B j):
-    ⊢ ith_sig i s -∗ smap_repr B m smap -∗
-      ex_ith_sig B i s ∗ (ex_ith_sig B' i s -∗ smap_repr B' m smap).
-  Proof using LEQUIV__l DISCR__l DISCR__d.
-    iIntros "#ITH SR".
-    iDestruct (ith_sig_in with "[$] [$]") as "%ITH".
-    rewrite /smap_repr. iDestruct "SR" as "(SM & % & SR)".
-    rewrite {2 5}(map_split smap i) ITH /=.
-    rewrite !big_sepM_union.
-    2: apply map_disjoint_singleton_l_2; by apply lookup_delete.
-    iDestruct "SR" as "[S SR]". rewrite !big_sepM_singleton.
-    iFrame.
-    2: { apply map_disjoint_dom. set_solver. }
-    iIntros. iSplitR; [done| ]. iFrame.
-    iApply (big_sepM_impl with "[$]"). iIntros "!> %% %OTHER".
-    apply lookup_delete_Some in OTHER as [? ?%mk_is_Some%elem_of_dom]. 
-    rewrite /ex_ith_sig. rewrite OTHER_PRES; [by iIntros; iFrame| ..]; done. 
-  Qed.
-
-  (* TODO: use bupd in definition of OU *)
-  Lemma smap_create_ep i B K smap π π__cp τ d__h d__l
-    (PH_LE: phase_le π__cp π)
-    (LT: i < K)
-    (DEG_LT: deg_lt d__l d__h):
-    ⊢ smap_repr B K smap -∗ 
-      cp π__cp d__h (oGS := oGS) -∗
-      th_phase_ge τ π (oGS := oGS) -∗
-      |==> OU (∃ s, ith_sig i s ∗
-                    ep s π__cp d__l (oGS := oGS) ∗ smap_repr B K smap ∗
-                    th_phase_ge τ π (oGS := oGS)) (oGS := oGS).
-  Proof using DISCR__d DISCR__l LEQUIV__l.
-    iIntros "SR CP PH".
-    rewrite /smap_repr. iDestruct "SR" as "(AUTH & %DOM & SIGS)".
-    assert (i ∈ dom smap) as [s ITH]%elem_of_dom.
-    { rewrite DOM. apply elem_of_set_seq. lia. }
-    rewrite {2 5}(map_split smap i) ITH /=.
-    setoid_rewrite big_sepM_union.
-    2, 3: apply map_disjoint_singleton_l_2; by apply lookup_delete.
-    iDestruct "SIGS" as "[SIG SIGS]". setoid_rewrite big_sepM_singleton.
-    rewrite {1}/ex_ith_sig. 
-    iDestruct (create_ep_upd with "CP [$] [PH]") as "OU".
-    { eauto. }
-    { done. }
-    { done. }
-    iMod (own_update with "AUTH") as "X". 
-    { apply auth_update_dfrac_alloc. 
-      2: { apply singleton_included_l with (i := i).
-           rewrite lookup_fmap ITH. eexists. split; [| reflexivity].
-           simpl. reflexivity. }
-      apply _. }
-    iApply (OU_wand with "[-OU]"); [| by iFrame].
-    iIntros "(EP & SIG & PH)".
-    iDestruct "X" as "[? ITH]". 
-    iExists _. iFrame. done.
-  Qed.
-
-  (* TODO: move, find existing? *)
-  Lemma lookup_delete_ne' `{Countable K} {V: Type} (k: K) (m: gmap K V)
-    (NOk: k ∉ dom m):
-    delete k m = m.
-  Proof using.
-    apply map_eq. intros.
-    destruct (decide (i = k)) as [-> | ?].
-    - rewrite lookup_delete. symmetry.
-      by apply not_elem_of_dom.
-    - by apply lookup_delete_ne.
-  Qed.                          
-
-  Lemma smap_sgns_extend (B B': nat -> bool)
-    (smap: gmap nat SignalId) (s : SignalId) (m : nat) (* lm *)
-    (DOM: dom smap = set_seq 0 m)
-    (PRES: forall i, i ∈ dom smap -> B' i = B i)
-    (* (LVL: lvl2nat lm = m) *)
-    :
-    ⊢ ([∗ map] k↦y ∈ smap, sgn y (L k) (Some (B k)) (oGS := oGS)) -∗
-       sgn s (L m) (Some (B' m)) (oGS := oGS) -∗
-       [∗ map] i↦s0 ∈ <[m := s]> smap, sgn s0 (L i) (Some $ B' i) (oGS := oGS).
-  Proof using.
-    iIntros "SIGS SG".
-    rewrite big_opM_insert_delete. 
-    iSplitL "SG"; [done| ].
-    rewrite lookup_delete_ne'.
-    2: { rewrite DOM. intros ?%elem_of_set_seq. lia. }
-    iApply (big_sepM_impl with "[$]"). iModIntro.
-    iIntros (??) "% ?".
-    rewrite PRES; [done| ].
-    eapply elem_of_dom; eauto. 
-    (* apply lookup_delete_Some in H0 as [??]. *)
-    (* apply mk_is_Some, elem_of_dom in H1. *)
-    (* rewrite DOM in H1. apply elem_of_set_seq in H1. *)
-    (* assert ((k <? m) = (k <? m + 1) \/ k = m). *)
-    (* { destruct (decide (k = m)); [tauto| ]. left. *)
-    (*   destruct (k <? m) eqn:LT. *)
-    (*   - rewrite (proj2 (PeanoNat.Nat.ltb_lt _ _)); [done | ]. *)
-    (*     apply PeanoNat.Nat.ltb_lt in LT. lia. *)
-    (*   - rewrite (proj2 (PeanoNat.Nat.ltb_ge _ _)); [done | ]. *)
-    (*     apply PeanoNat.Nat.ltb_ge in LT. lia. } *)
-    (* destruct H2; [| done]. rewrite H2. done. *)
-  Qed.
-
-  (* Lemma smap_sgns_extend (B0: nat -> nat -> bool) *)
-  (*   (smap: gmap nat SignalId) (s : SignalId) (m : nat) (* lm *) *)
-  (*   (DOM: dom smap = set_seq 0 m) *)
-  (*   (PRES: forall i, i ∈ dom smap -> B0 (m + 1) i = B0 m i) *)
-  (*   (* (LVL: lvl2nat lm = m) *) *)
-  (*   : *)
-  (*   ⊢ ([∗ map] k↦y ∈ smap, sgn y (L k) (Some (B0 m k)) (oGS := oGS)) -∗ *)
-  (*      sgn s (L m) (Some (B0 (m + 1) m)) (oGS := oGS) -∗ *)
-  (*      [∗ map] i↦s0 ∈ <[m := s]> smap, sgn s0 (L i) (Some $ B0 (m + 1) i) (oGS := oGS). *)
-  (* Proof using. *)
-  (*   iIntros "SIGS SG". *)
-  (*   rewrite big_opM_insert_delete.  *)
-  (*   iSplitL "SG"; [done| ]. *)
-  (*   rewrite lookup_delete_ne'. *)
-  (*   2: { rewrite DOM. intros ?%elem_of_set_seq. lia. } *)
-  (*   iApply (big_sepM_impl with "[$]"). iModIntro. *)
-  (*   iIntros (??) "% ?". *)
-  (*   rewrite PRES; [done| ]. *)
-  (*   eapply elem_of_dom; eauto.  *)
-  (*   (* apply lookup_delete_Some in H0 as [??]. *) *)
-  (*   (* apply mk_is_Some, elem_of_dom in H1. *) *)
-  (*   (* rewrite DOM in H1. apply elem_of_set_seq in H1. *) *)
-  (*   (* assert ((k <? m) = (k <? m + 1) \/ k = m). *) *)
-  (*   (* { destruct (decide (k = m)); [tauto| ]. left. *) *)
-  (*   (*   destruct (k <? m) eqn:LT. *) *)
-  (*   (*   - rewrite (proj2 (PeanoNat.Nat.ltb_lt _ _)); [done | ]. *) *)
-  (*   (*     apply PeanoNat.Nat.ltb_lt in LT. lia. *) *)
-  (*   (*   - rewrite (proj2 (PeanoNat.Nat.ltb_ge _ _)); [done | ]. *) *)
-  (*   (*     apply PeanoNat.Nat.ltb_ge in LT. lia. } *) *)
-  (*   (* destruct H2; [| done]. rewrite H2. done. *) *)
-  (* Qed.
- *)
-  Lemma BMU_smap_extend `{invGS_gen HasNoLc Σ} τ m smap R
-    (* B0 *)
-    (B B': nat -> bool)
-    (PRES: forall i, i ∈ dom smap -> B' i = B i)
-    (FRESH_UNSET: B' m = false):
-    ⊢ obls τ R (oGS := oGS) -∗ smap_repr B m smap -∗
-      BMU ∅ 1 (
-        |==> (∃ s',
-             smap_repr B' (m + 1) (<[m := s']> smap) ∗
-             ith_sig m s' ∗ obls τ (R ∪ {[s']}) (oGS := oGS) ∗
-             ⌜ s' ∉ R ⌝)) (oGS := oGS).
-    Proof using LEQUIV__l DISCR__l DISCR__d.
-      iIntros "OBLS SM".
-      iApply OU_BMU.
-      iDestruct (OU_create_sig with "OBLS") as "FOO".
-      iApply (OU_wand with "[-FOO]"); [| by iFrame].
-      iIntros "(%s' & SG & OBLS & %NEW)".
-      iApply BMU_intro.
-      rewrite /smap_repr. iDestruct "SM" as "(SM & %DOM & SIGS)". 
-      iMod (own_update with "SM") as "SM".
-      { apply auth_update_alloc. eapply (alloc_singleton_local_update _ m (to_agree s')).
-        2: done.
-        apply not_elem_of_dom. rewrite dom_fmap. rewrite DOM.
-        intros ?%elem_of_set_seq. lia. }
-      iModIntro. iDestruct "SM" as "[SM S']".
-      iExists s'.
-      rewrite -fmap_insert. iFrame. iSplit; [| done].
-      iSplitR.
-      { iPureIntro. rewrite dom_insert_L.
-        rewrite set_seq_add_L. rewrite -DOM. set_solver. }
-      iApply (smap_sgns_extend with "[$]"); try done.
-      rewrite FRESH_UNSET. iFrame.
-    Qed.
-      
-  (*   Lemma BMU_smap_restore τ s m smap *)
-  (*     (DOM : dom smap = set_seq 0 (B `min` (m + 2))) *)
-  (*     (IN : smap !! m = Some s) *)
-  (*     (lm : sigO (λ i : nat, i < LIM)) *)
-  (*     (LVL : lvl2nat lm = m): *)
-  (*       ⊢ *)
-  (* obls τ ∅ (oGS := oGS) -∗ *)
-  (* ([∗ map] k↦y ∈ delete m smap, ∃ l0 : sigO (λ i : nat, i < LIM), *)
-  (*                                         sgn y l0 (Some (k <? m)) (oGS := oGS) ∗ *)
-  (*                                         ⌜lvl2nat l0 = k⌝) -∗ *)
-  (* (sgn s lm (Some true) (oGS := oGS)) -∗ *)
-  (* own eofin_smap (● ((to_agree <$> smap): gmap _ _)) -∗ *)
-  (* BMU (⊤ ∖ ↑nroot.@"eofin") 1 *)
-  (*   (⌜B ≤ m + 2⌝ ∗ obls τ ∅ (oGS := oGS) ∗ smap_repr_eo (B `min` (m + 2)) (m + 1) smap *)
-  (*    ∨ (|==> ⌜m + 2 < B⌝ ∗ *)
-  (*         (∃ (s' : SignalId) (lm': EOLevel B), *)
-  (*            smap_repr_eo (B `min` (m + 3)) (m + 1) (<[m + 2:=s']> smap) ∗ *)
-  (*            ith_sig (m + 2) s' ∗ obls τ {[s']} (oGS := oGS) ∗ *)
-  (*            ⌜lvl2nat lm' = (m + 2)%nat⌝))) (oGS := oGS). *)
-  (*   Proof using. *)
-  (*     iIntros "OBLS SIGS SIG SM". *)
-  (*     destruct (Nat.le_gt_cases B (m + 2)). *)
-  (*     { rewrite PeanoNat.Nat.min_l in DOM; [| done].  *)
-  (*       iApply BMU_intro. iLeft. iFrame. *)
-  (*       iSplitR; [done| ]. iSplitR. *)
-  (*       { iPureIntro. rewrite PeanoNat.Nat.min_l; auto. } *)
-  (*       iApply (restore_map with "[$] [$]"); eauto. *)
-  (*       rewrite DOM. f_equal. symmetry. by apply Nat.min_l. } *)
-      
-  (*     iApply OU_BMU. *)
-  (*     assert {lm' : EOLevel B | lvl2nat lm' = m + 2} as [lm' LVL']. *)
-  (*     { set (lm' := exist _ (m + 2) H0: EOLevel B). *)
-  (*       exists lm'. done. } *)
-  (*     iDestruct (OU_create_sig with "OBLS") as "FOO". *)
-  (*     iApply (OU_wand with "[-FOO]"); [| by iFrame]. *)
-  (*     iIntros "(%s' & SG & OBLS & %NEW)". rewrite union_empty_l_L. *)
-  (*     iApply BMU_intro. iRight. iSplitR; [done| ]. *)
-  (*     rewrite PeanoNat.Nat.min_r in DOM; [| lia]. *)
-  (*     iMod (own_update with "SM") as "SM". *)
-  (*     { apply auth_update_alloc. eapply (alloc_singleton_local_update _ (m + 2) (to_agree s')). *)
-  (*       2: done.  *)
-  (*       apply not_elem_of_dom. rewrite dom_fmap. rewrite DOM. *)
-  (*       intros ?%elem_of_set_seq. lia. } *)
-  (*     iModIntro. iDestruct "SM" as "[SM S']". *)
-  (*     iExists s', lm'.  *)
-  (*     iSplitL "SIGS SG SIG SM". *)
-  (*     2: { iFrame. eauto. } *)
-  (*     rewrite PeanoNat.Nat.min_r; [| lia]. rewrite /smap_repr_eo. *)
-  (*     rewrite -fmap_insert. iFrame. iSplitR. *)
-  (*     { iPureIntro. rewrite dom_insert_L DOM. *)
-  (*       apply set_eq. intros ?. rewrite elem_of_union elem_of_singleton. *)
-  (*       rewrite !elem_of_set_seq. lia. } *)
-  (*     rewrite big_sepM_insert_delete. iSplitL "SG". *)
-  (*     { iExists _. rewrite (proj2 (PeanoNat.Nat.ltb_ge _ _)); [ | lia]. *)
-  (*       iFrame. iPureIntro. *)
-  (*       Unshelve. *)
-  (*       2: { assert (m + 2 < LIM) by lia.  *)
-  (*            esplit. apply H1. } *)
-  (*       done. } *)
-  (*     rewrite (delete_notin _ (m + 2)). *)
-  (*     2: { apply not_elem_of_dom. rewrite DOM. intros ?%elem_of_set_seq. lia. } *)
-  (*     iApply (restore_map with "[$] [$]"); eauto. *)
-  (*     rewrite DOM. f_equal. symmetry. lia. *)
-  (*   Qed. *)
-
-    Lemma ith_sig_expect i sw m τ π π__e smap R d B
-      (PH_EXP: phase_le π__e π)
-      (GE: m <= i)
-      (UNSETi: B i = false):
-      ⊢ ep sw π__e d (oGS := oGS) -∗ th_phase_ge τ π (oGS := oGS) -∗
-         smap_repr B m smap -∗ ith_sig i sw -∗
-         obls τ R (oGS := oGS) -∗ sgns_level_gt R (L i) (oGS := oGS) -∗ 
-         OU (∃ π', cp π' d (oGS := oGS) ∗ smap_repr B m smap ∗ th_phase_ge τ π' (oGS := oGS) ∗ obls τ R (oGS := oGS) ∗ ⌜ phase_le π π' /\ phase_le π__e π' ⌝) (oGS := oGS).
-    Proof using LEQUIV__l DISCR__l.
-      iIntros "#EP PH SR #SW OBLS #OBLS_LT". 
-      iDestruct (ith_sig_in with "[$] [$]") as "%ITH".
-      iDestruct (smap_repr_split with "SW [$]") as "[SGw SR]".
-      rewrite {1}/ex_ith_sig. rewrite UNSETi. 
-      iDestruct (expect_sig_upd with "EP [$] [$] [$] [$]") as "OU"; [done| ..].
-      iApply (OU_wand with "[-OU]"); [| done].
-      iIntros "(%π' & CP1 & SIGW & OBLS & PH & [%PH_LE' %PH_LE''])".
-      iExists _. iFrame. iSplitL; [| done].
-      iApply "SR". rewrite /ex_ith_sig. by rewrite UNSETi.
-    Qed.
-
-    Lemma smap_expose_dom B m smap:
-      ⊢ smap_repr B m smap -∗ ⌜ dom smap = set_seq 0 m ⌝.
-    Proof using. by iIntros "(?&?&?)". Qed.
-
-End SignalMap.
 
 Section EoFin.
   Context (B: nat).
@@ -402,17 +60,13 @@ Section EoFin.
   Class EoFinPreG Σ := {
       eofin_threads_PreG :> inG Σ (excl_authR natO);
       eofin_sigs :> SigMapPreG Σ;
-        (* inG Σ (authUR (gmapUR nat (agreeR SignalId))); *)                 
   }.
   
   Class EoFinG Σ := {
       eofin_PreG :> EoFinPreG Σ;
       eofin_even: gname; eofin_odd: gname;
-      (* eofin_smap: gname; *)
       eofin_sm :> SigMapG Σ;
   }.
-
-  Definition lvl2nat {X} (l: EOLevel X) := bn2nat _ l. 
 
   Definition d0 := ith_bn NUM_DEG 0 ltac:(lia).
   Definition d1 := ith_bn NUM_DEG 1 ltac:(lia). 
@@ -503,37 +157,6 @@ Section EoFin.
     Definition eofin_inv l: iProp Σ :=
       inv (nroot .@ "eofin") (eofin_inv_inner l).
 
-    (* Lemma restore_map (smap: gmap nat SignalId) (s : SignalId) (m : nat) lm *)
-    (*   (DOM: dom smap = set_seq 0 (B `min` (m + 2))) *)
-    (*   (IN: smap !! m = Some s) *)
-    (*   (LVL: lvl2nat lm = m) *)
-    (*   : *)
-    (*   ⊢ (([∗ map] k↦y ∈ delete m smap, *)
-    (*        ∃ l0, sgn y l0 (Some (k <? m)) (oGS := oGS) ∗ ⌜lvl2nat l0 = k⌝) -∗ *)
-    (*       sgn s lm (Some true) (oGS := oGS)-∗ *)
-    (*       [∗ map] i↦s0 ∈ smap, *)
-    (*        ∃ l0, sgn s0 l0 (Some (i <? m + 1)) (oGS := oGS) ∗ ⌜ lvl2nat l0 = i⌝)%I. *)
-    (* Proof using. *)
-    (*   iIntros "SIGS SG". *)
-    (*   rewrite (big_sepM_delete _ smap); eauto. *)
-    (*   iSplitL "SG". *)
-    (*   { iExists _. rewrite (proj2 (Nat.ltb_lt _ _)); [| lia]. *)
-    (*     iFrame. done. } *)
-    (*   iApply (big_sepM_impl with "[$]"). iModIntro. *)
-    (*   iIntros (???) "(%&?&?)". iExists _. iFrame. *)
-    (*   apply lookup_delete_Some in H0 as [??]. *)
-    (*   apply mk_is_Some, elem_of_dom in H1. *)
-    (*   rewrite DOM in H1. apply elem_of_set_seq in H1. *)
-    (*   assert ((k <? m) = (k <? m + 1) \/ k = m). *)
-    (*   { destruct (decide (k = m)); [tauto| ]. left. *)
-    (*     destruct (k <? m) eqn:LT. *)
-    (*     - rewrite (proj2 (PeanoNat.Nat.ltb_lt _ _)); [done | ]. *)
-    (*       apply PeanoNat.Nat.ltb_lt in LT. lia. *)
-    (*     - rewrite (proj2 (PeanoNat.Nat.ltb_ge _ _)); [done | ]. *)
-    (*       apply PeanoNat.Nat.ltb_ge in LT. lia. } *)
-    (*   destruct H2; [| done]. rewrite H2. done. *)
-    (* Qed. *)
-
     (* TODO: generalize, move *)
     Lemma lvl_lt_equiv (l1 l2: EOLevel LIM):
       lvl_lt l1 l2 <-> bn2nat _ l1 < bn2nat _ l2.
@@ -555,27 +178,6 @@ Section EoFin.
     }.
 
     Lemma lt_B_LIM: B < LIM. lia. Qed. 
-
-  (*   Lemma BMU_smap_restore τ s m smap *)
-  (*     (DOM : dom smap = set_seq 0 (B `min` (m + 2))) *)
-  (*     (IN : smap !! m = Some s) *)
-  (*     (lm : sigO (λ i : nat, i < LIM)) *)
-  (*     (LVL : lvl2nat lm = m): *)
-  (*       ⊢ *)
-  (* obls τ ∅ (oGS := oGS) -∗ *)
-  (* ([∗ map] k↦y ∈ delete m smap, ∃ l0 : sigO (λ i : nat, i < LIM), *)
-  (*                                         sgn y l0 (Some (k <? m)) (oGS := oGS) ∗ *)
-  (*                                         ⌜lvl2nat l0 = k⌝) -∗ *)
-  (* (sgn s lm (Some true) (oGS := oGS)) -∗ *)
-  (* own eofin_smap (● ((to_agree <$> smap): gmap _ _)) -∗ *)
-  (* BMU (⊤ ∖ ↑nroot.@"eofin") 1 *)
-  (*   (⌜B ≤ m + 2⌝ ∗ obls τ ∅ (oGS := oGS) ∗ smap_repr_eo (B `min` (m + 2)) (m + 1) smap *)
-  (*    ∨ (|==> ⌜m + 2 < B⌝ ∗ *)
-  (*         (∃ (s' : SignalId) (lm': EOLevel B), *)
-  (*            smap_repr_eo (B `min` (m + 3)) (m + 1) (<[m + 2:=s']> smap) ∗ *)
-  (*            ith_sig (m + 2) s' ∗ obls τ {[s']} (oGS := oGS) ∗ *)
-  (*            ⌜lvl2nat lm' = (m + 2)%nat⌝))) (oGS := oGS). *)
-
 
     Lemma BMU_update_SR smap τ m:
   obls τ ∅ (oGS := oGS) -∗
@@ -610,12 +212,18 @@ Section EoFin.
       Unshelve. apply _.
     Qed.
 
+    Lemma B__eo_simpl i (DOM: i < LIM):
+      B__eo i = ith_bn LIM i DOM.
+    Proof.      
+      rewrite /B__eo. destruct le_lt_dec; [lia| ].
+      f_equal. eapply Nat.lt_pi.
+    Qed.
+
     Lemma thread_spec_holds τ l (π π2: Phase) n
       (PH_LE2: phase_le π2 π)
       `(ThreadResource th_res cond)
       :
       {{{ eofin_inv l ∗ exc_lb 20 (oGS := oGS) ∗
-           (* even_res n ∗ *)
            th_res n ∗
            cp_mul π2 d2 (B - n) (oGS := oGS) ∗
            cp_mul π d0 20 (oGS := oGS) ∗
@@ -662,14 +270,9 @@ Section EoFin.
         { econstructor. done. }
         iNext. iIntros "L".
         
-        (* iDestruct (ith_sig_in with "[$] [$]") as %IN. *)
-        (* iDestruct "SR" as "(SM & %DOM & SIGS)". *)
-        
-        (* iDestruct (big_sepM_delete with "SIGS") as "[SG SIGS]"; eauto. *)
-        (* iDestruct "SG" as (lm) "(SG & %LVL)". *)
         iDestruct (smap_expose_dom with "[$]") as "%SM_DOM". 
         rewrite /smap_repr_eo. 
-        
+
         iPoseProof (smap_repr_split_upd B__eo _ (flip Nat.ltb (m + 1)) with "[$] [$]") as "[SG SR_CLOS]".
         { intros ?. rewrite SM_DOM elem_of_set_seq. simpl.
           intros NEQ [? [??]%Nat.min_glb_lt_iff].
@@ -684,7 +287,6 @@ Section EoFin.
         iApply (OU_wand with "[-OU]"); [| done]. iIntros "(SIG & OBLS)".
         rewrite (subseteq_empty_difference_L {[ s ]}); [| done].
         
-        (* iPoseProof (BMU_smap_restore with "OBLS [$] [$] [$]") as "BMU"; eauto. *)
         iSpecialize ("SR_CLOS" with "[SIG]").
         { rewrite /ex_ith_sig. simpl.
           rewrite !(proj2 (PeanoNat.Nat.ltb_lt _ _)); [iFrame | lia]. }
@@ -709,7 +311,6 @@ Section EoFin.
           
           iMod ("CLOS" with "[AUTH SR L]") as "?".
           { rewrite /eofin_inv_inner. iNext. iExists (m + 1), smap.
-            (* rewrite even_plus1_negb odd_plus1_negb E -O. simpl.  *)
             rewrite -Nat.add_assoc. rewrite Nat2Z.inj_add. 
             iFrame. }
           
@@ -730,11 +331,9 @@ Section EoFin.
         + iDestruct "COND" as "[CC | COND]".
           { iDestruct "CC" as "(% & % & %)". lia. }
           iClear "SN".  
-          (* iMod "COND" as "[% (%s' & %lm' & SM & SN & OBLS & %LVL')]".  *)
           iDestruct "COND" as "(%s'& SN & (%LT & -> & ->))".
           iMod ("CLOS" with "[AUTH SR L]") as "?".
           { rewrite /eofin_inv_inner. iNext. iExists (m + 1), _.
-            (* rewrite even_plus1_negb odd_plus1_negb E -O. simpl.  *)
             rewrite -Nat.add_assoc. rewrite Nat2Z.inj_add. 
             iFrame. }
           
@@ -792,14 +391,18 @@ Section EoFin.
           iMod (smap_create_ep B__eo m with "[$] [$] [$]") as "OU"; eauto.
           { lia. }
           { apply d12_lt. }
+          Unshelve. 2: by apply _.
           iApply OU_BMU.
           iApply (OU_wand with "[-OU]"); [| done]. iIntros "(%sw & #SW & #EP & SR & PH)".
-          (* rewrite -E in H0. *)
-
-          foobar. 
-          iDestruct (ith_sig_expect B__eo with "[$] [$] [$] [$] [$] [$]") as "OU".
+          iDestruct (ith_sig_sgn with "SN [$]") as "#EX". 
+          iDestruct (ith_sig_expect B__eo with "[$] [$] [$] SW [$] []") as "OU".
           { done. }
-          { reflexivity. }
+          { apply Nat.ltb_irrefl. }
+          { rewrite /sgns_level_gt. rewrite big_opS_singleton.
+            iExists _. iFrame "EX". iPureIntro.
+            rewrite !B__eo_simpl; try lia. intros.
+            apply ith_bn_lt. lia. }
+            
           iApply OU_BMU.
           iApply (OU_wand with "[-OU]"); [| done].
           iIntros "(%π' & CP1 & SR & PH & OBLS & [%PH_LE' %])".
@@ -835,9 +438,14 @@ Section EoFin.
         + MU_by_BMU. 
           iDestruct "EXP" as "(%sw & %π__e & #SW & #EP & %PH_EXP)".
           rewrite Nat.add_sub.
-          iDestruct (ith_sig_expect with "[$] [$] [$] [$] [$] [$]") as "OU".
+          iDestruct (ith_sig_sgn with "SN [$]") as "#EX". 
+          iDestruct (ith_sig_expect B__eo with "[$] [$] [$] [$] [$] []") as "OU".
           { apply PH_EXP. }
-          { reflexivity. }
+          { apply Nat.ltb_irrefl. }
+          { rewrite /sgns_level_gt. rewrite big_opS_singleton.
+            iExists _. iFrame "EX". iPureIntro.
+            rewrite !B__eo_simpl; try lia. intros.
+            apply ith_bn_lt. lia. }
           iApply OU_BMU.
           iApply (OU_wand with "[-OU]"); [| done].
           iIntros "(%π' & CP1 & SR & PH & OBLS & [%PH_LE' %PH_LE''])".
@@ -866,7 +474,7 @@ Section EoFin.
                iExists _. iFrame "#∗". }
           iRight. rewrite Nat.add_sub.
           do 2 iExists _. iFrame "#∗". done.
-    Time Qed. 
+    Time Qed.
 
     Lemma thread_spec_wrapper τ l (π π2: Phase) n
       (PH_LE2: phase_le π2 π)
@@ -937,39 +545,6 @@ Section EoFin.
       done.
     Qed.
 
-    Definition sigs_block (smap: gmap nat SignalId) from len: list SignalId :=
-      map (fun k => default 0 (smap !! k)) (seq from len).
-
-    Lemma sigs_block_in smap from len:
-      forall s i, smap !! i = Some s -> i ∈ seq from len -> s ∈ sigs_block smap from len.
-    Proof using.
-      intros ?? ITH DOM. rewrite /sigs_block.
-      apply elem_of_list_In. apply in_map_iff. setoid_rewrite <- elem_of_list_In. 
-      eexists. split; eauto. by rewrite ITH.
-    Qed.
-
-    Lemma sigs_block_len smap from len: length $ sigs_block smap from len = len.
-    Proof using.
-      rewrite /sigs_block. by rewrite map_length seq_length.
-    Qed.
-
-    Lemma sigs_block_is_Some smap from len:
-      forall k, is_Some (sigs_block smap from len !! k) <-> k < len.
-    Proof using.
-      intros. 
-      rewrite lookup_lt_is_Some. by rewrite sigs_block_len.
-    Qed.
-
-    Lemma sigs_block_lookup_eq smap from len:
-      forall k, k < len -> from + k ∈ dom smap -> sigs_block smap from len !! k = smap !! (from + k). 
-    Proof using.
-      intros ? DOMsb DOMm.
-      rewrite /sigs_block.
-      rewrite list_lookup_fmap.
-      rewrite lookup_seq_lt; [| done]. simpl.
-      apply elem_of_dom in DOMm as [? DOMm]. by rewrite DOMm.
-    Qed. 
-
     (* TODO: parametrize smap_repr_eo with the lower bound *)
     Lemma alloc_inv l (* (i: nat) *) τ
       (* (i := 0) *)
@@ -991,17 +566,14 @@ Section EoFin.
       
       set (m := min B 2).
       iAssert (BMU ⊤ 2 
-                 (|==> ∃ γ smap, smap_repr_eo' γ m 0 smap ∗
-                                 (* let sigs := map_img smap in *)
-                                 let sigs := sigs_block smap 0 m in
-                                 obls τ (list_to_set sigs) (oGS := oGS) ∗
-                                 (* ⌜ size sigs = m ⌝ ∗ *)
-                                  ⌜ NoDup sigs ⌝ ∗ 
-                                 own γ (◯ ((to_agree <$> smap): gmapUR nat _))
+                 (|==> ∃ smap (smG: SigMapG Σ), smap_repr B__eo (flip Nat.ltb 0) m smap ∗
+                               let sigs := sigs_block smap 0 m in
+                               obls τ (list_to_set sigs) (oGS := oGS) ∗
+                               ⌜ NoDup sigs ⌝ ∗ 
+                               own sm_γ__smap (◯ ((to_agree <$> smap): gmapUR nat _)) ∗
+                               ⌜ @sm_PreG _ smG = @eofin_sigs _ PRE ⌝
               ))%I with "[OB]" as "-#SR".
-      {
-        
-        assert (m <= 0 \/ m = 0 + 1 \/ m = 0 + 2) as [LE | [EQ | EQ]] by lia; revgoals.
+      { assert (m <= 0 \/ m = 0 + 1 \/ m = 0 + 2) as [LE | [EQ | EQ]] by lia; revgoals.
         - iApply OU_BMU.
           assert (0 < LIM) as Di by lia. 
           unshelve iDestruct (OU_create_sig with "[$]") as "OU".
@@ -1018,11 +590,12 @@ Section EoFin.
           set (smap0 := {[ 0 := si; 0 + 1 := si']}: gmap nat SignalId).
           iMod (own_alloc (● ((to_agree <$> smap0): gmapUR nat (agreeR SignalId)) ⋅ ◯ _)) as (?) "[A F]".
           { apply auth_both_valid_2; [| reflexivity]. apply map_nat_agree_valid. }
-          iModIntro. iExists _, _. iFrame. 
+          iModIntro.
+          iExists _, {| sm_γ__smap := γ0|}. iFrame. 
           replace (sigs_block smap0 0 m) with ([ si; si' ]).
           2: { subst smap0 m. rewrite EQ. rewrite /sigs_block. simpl. done. } 
 
-          rewrite !bi.sep_assoc. iSplitL.
+          rewrite !bi.sep_assoc. iSplitL; [| done]. iSplitL. 
           2: { iPureIntro. econstructor; try set_solver. apply NoDup_singleton. }
           
           iSplitR "OBLS".
@@ -1035,11 +608,8 @@ Section EoFin.
             rewrite EQ. simpl. set_solver. }
           subst smap0. rewrite !big_sepM_insert; try set_solver.
           rewrite big_sepM_empty. rewrite /ex_ith_sig.
-          rewrite bi.sep_assoc. iSplitL; [| done]. iSplitL "SGi".
-          + iExists _. rewrite (proj2 (PeanoNat.Nat.ltb_ge _ _)); [| lia].
-            iFrame. done. 
-          + iExists _. rewrite (proj2 (PeanoNat.Nat.ltb_ge _ _)); [| lia].
-            iFrame. done.
+          simpl. rewrite !(proj2 (PeanoNat.Nat.ltb_ge _ _)); try lia.
+          rewrite !B__eo_simpl. iFrame.
         - iApply OU_BMU.
           assert (0 < LIM) as Di by lia. 
           unshelve iDestruct (OU_create_sig with "[$]") as "OU".
@@ -1050,11 +620,12 @@ Section EoFin.
           set (smap0 := {[ 0 := si]}: gmap nat SignalId).
           iMod (own_alloc (● ((to_agree <$> smap0): gmapUR nat (agreeR SignalId)) ⋅ ◯ _)) as (?) "[A F]".
           { apply auth_both_valid_2; [| reflexivity]. apply map_nat_agree_valid. }
-          iModIntro. iExists _, _. iFrame.
+          iModIntro. iExists _, {| sm_γ__smap := γ0 |}. iFrame.
           replace (sigs_block smap0 0 m) with [si].
           2: { subst smap0 m. rewrite EQ. rewrite /sigs_block. simpl. done. }
           iSplitR "OBLS".
-          2: { iSplitL; [| iPureIntro; by apply NoDup_singleton]. 
+          2: { iSplitL.
+               2: { iSplit; [| done]. iPureIntro. by apply NoDup_singleton. }
                iApply obls_proper; [| by iFrame]. set_solver. }
 
           iSplitR.
@@ -1063,21 +634,19 @@ Section EoFin.
             rewrite EQ. simpl. set_solver. }
           subst smap0. rewrite !big_sepM_insert; try set_solver.
           rewrite big_sepM_empty. rewrite /ex_ith_sig.
-          iSplitL; [| done].
-          iExists _. rewrite (proj2 (PeanoNat.Nat.ltb_ge _ _)); [| lia].
-          iFrame. done.
+          simpl. rewrite !(proj2 (PeanoNat.Nat.ltb_ge _ _)); try lia.
+          rewrite !B__eo_simpl. iFrame.
         - iApply BMU_intro.
           set (smap0 := ∅: gmap nat SignalId).
           iMod (own_alloc (● ((to_agree <$> smap0): gmapUR nat (agreeR SignalId)) ⋅ ◯ _)) as (?) "[A F]".
           { apply auth_both_valid_2; [| reflexivity]. apply map_nat_agree_valid. }
-          iModIntro. iExists _, _. iFrame.
+          iModIntro. iExists _, {| sm_γ__smap := γ0 |}. iFrame.
           assert (B = 0) by lia. simpl.  
           replace (sigs_block smap0 0 m) with (nil: list SignalId).
           2: { subst smap0 m. simpl. rewrite H. done. }
 
           iSplitR "OB".
-          2: { iFrame. iPureIntro; constructor. }
-          rewrite /smap_repr_eo'. iFrame.
+          2: { iFrame. iPureIntro. split; done || constructor. }
           iSplitR.
           { subst smap0. iPureIntro. 
             subst m. (* subst i. *)
@@ -1085,14 +654,12 @@ Section EoFin.
           subst smap0. rewrite big_sepM_empty. done. }
 
       iApply (BMU_wand with "[-SR] [$]"). 
-      iIntros "X". iMod "X" as "(%γ__sr & %smap & SR & OB & %SIZE & #F)".
+      iIntros "X". iMod "X" as "(%smap & %SMG & SR & OB & %SIZE & #F & %EQ_PRE)".
       
       set (eoG := {| 
-          (* eofin_even := (if Nat.even i then γ else γ'); *)
-          (* eofin_odd := (if Nat.even i then γ' else γ); *)
           eofin_even := (if Nat.even 0 then γ else γ');
           eofin_odd := (if Nat.even 0 then γ' else γ);
-          eofin_smap := γ__sr
+          eofin_sm := SMG;
       |}).
       
       iExists eoG, _. iFrame.
@@ -1109,6 +676,8 @@ Section EoFin.
       2: { simpl. rewrite DOM. apply elem_of_set_seq. lia. }
       simpl in IN.       
       rewrite /ith_sig.
+      (* Set Printing Implicit. simpl. *)
+      rewrite EQ_PRE. 
       iApply (own_mono with "F").
       apply auth_frag_mono.
       apply singleton_included_l. eexists.
@@ -1347,7 +916,6 @@ Section EoFin.
         iIntros "[? (%π1 & %π2 & PH1 & OB1 & PH3 & OB2 & [%LT1 %LT2])]".
         Unshelve. 2: exact ∅.
 
-
         rewrite difference_diag_L. rewrite intersection_idemp_L.
         iSplitL "RE CPS2 CPS_FORK PH3 OB2".
         { iApply (thread_spec_wrapper with "[-]").
@@ -1394,7 +962,6 @@ Section EoFin.
         { apply odd_thread_resource. }
         2: { iNext. iIntros (v) "OB". by iApply NO_OBS_POST. }
         simpl. 
-        (* iDestruct (cp_mul_take with "CPS2'") as "[CPS2 ?]".  *)        
         rewrite (proj2 (PeanoNat.Nat.ltb_ge _ _)); [| lia].
         rewrite {1 3}B0. simpl.  
         iFrame "CPS2'". iFrame "#∗".
