fairness/lawyer/examples/signal_map.v
@@ -1,0 +1,275 @@
+From iris.proofmode Require Import tactics coq_tactics.
+From iris.algebra Require Import auth gmap gset excl excl_auth.
+From trillium.fairness Require Import utils.
+From trillium.fairness.lawyer Require Import sub_action_em.
+From trillium.fairness.lawyer.obligations Require Import obligations_model obligations_resources obligations_logic obligations_em.
+
+Section SignalMap.
+
+  Class SigMapPreG Σ := {
+      sm_sig_map :> inG Σ (authUR (gmapUR nat (agreeR SignalId)));
+  }.
+  
+  Class SigMapG Σ := {
+      sm_PreG :> SigMapPreG Σ;
+      sm_γ__smap: gname;
+  }.
+
+  Context `{SigMapG Σ}.
+
+  Context `{DISCR__d: OfeDiscrete DegO} `{DISCR__l: OfeDiscrete LevelO}.
+  Context {LEQUIV__l: @LeibnizEquiv (ofe_car LevelO) (ofe_equiv LevelO)}.   
+  Let Degree := ofe_car DegO.
+  Let Level := ofe_car LevelO.
+  (* Context `{OP: ObligationsParams Degree Level Locale LIM_STEPS}. *)
+  Context `{OP': ObligationsParamsPre Degree Level LIM_STEPS}.
+  Let EO_OP := LocaleOP (Locale := locale heap_lang). 
+  Existing Instance EO_OP. 
+
+  Context {oGS: ObligationsGS Σ}.
+
+  Context (L: nat -> Level). 
+
+  Definition ex_ith_sig B (i: nat) (s: SignalId): iProp Σ :=
+    sgn s (L i) (Some $ B i) (oGS := oGS). 
+  
+  Definition smap_repr B K (smap: gmap nat SignalId): iProp Σ :=
+    own sm_γ__smap (● (to_agree <$> smap: gmapUR nat (agreeR SignalId))) ∗
+    ⌜ dom smap = set_seq 0 K ⌝ ∗
+    ([∗ map] i ↦ s ∈ smap, ex_ith_sig B i s).
+
+  Definition ith_sig (i: nat) (s: SignalId): iProp Σ :=
+    own sm_γ__smap (◯ {[ i := to_agree s ]}).
+
+  Lemma ith_sig_in i s B K (smap: gmap nat SignalId):
+    ⊢ ith_sig i s -∗ smap_repr B K smap -∗ ⌜ smap !! i = Some s ⌝.
+  Proof using.
+    iIntros "S (SM & ? & ?)". iCombine "SM S" as "SM".
+    iDestruct (own_valid with "SM") as %V.
+    apply auth_both_valid_discrete in V as [V ?].
+    apply singleton_included_l in V. destruct V as (x & ITH & LE).
+    iPureIntro.
+    rewrite Some_included_total in LE.
+    destruct (to_agree_uninj x) as [y X].
+    { eapply lookup_valid_Some; eauto. done. }
+    rewrite -X in LE. apply to_agree_included in LE.
+    rewrite -X in ITH.
+    
+    eapply leibniz_equiv.       
+    rewrite lookup_fmap in ITH.
+    rewrite -LE in ITH.
+    
+    apply fmap_Some_equiv in ITH as (?&ITH&EQ).
+    rewrite ITH. apply to_agree_inj in EQ. by rewrite EQ.
+  Qed.
+
+  Lemma ith_sig_sgn i s B K (smap: gmap nat SignalId):
+    ⊢ ith_sig i s -∗ smap_repr B K smap -∗ sgn s (L i) None (oGS := oGS).
+  Proof using.
+    iIntros "S SR".
+    iDestruct (ith_sig_in with "[$] [$]") as "%ITH". 
+    iDestruct "SR" as "(SM & % & ?)".
+    iDestruct (big_sepM_lookup with "[$]") as "ITH"; eauto.
+    rewrite /ex_ith_sig.     
+    by iDestruct (sgn_get_ex with "[$]") as "[??]". 
+  Qed.
+
+  Lemma smap_repr_split B K smap i s:
+    ⊢ ith_sig i s -∗ smap_repr B K smap -∗
+      ex_ith_sig B i s ∗ (ex_ith_sig B i s -∗ smap_repr B K smap).
+  Proof using.
+    iIntros "#ITH SR".
+    iDestruct (ith_sig_in with "[$] [$]") as "%ITH".
+    rewrite /smap_repr. iDestruct "SR" as "(SM & % & SR)".
+    rewrite {2 5}(map_split smap i) ITH /=.
+    rewrite !big_sepM_union.
+    2: apply map_disjoint_singleton_l_2; by apply lookup_delete.
+    iDestruct "SR" as "[S SR]". rewrite big_sepM_singleton.
+    iFrame. iIntros. iFrame. done.
+  Qed.
+
+  Lemma smap_repr_split_upd B B' m smap i s
+    (OTHER_PRES: forall j, j ≠ i -> j ∈ dom smap -> B' j = B j):
+    ⊢ ith_sig i s -∗ smap_repr B m smap -∗
+      ex_ith_sig B i s ∗ (ex_ith_sig B' i s -∗ smap_repr B' m smap).
+  Proof using.
+    clear LEQUIV__l DISCR__l DISCR__d.
+    iIntros "#ITH SR".
+    iDestruct (ith_sig_in with "[$] [$]") as "%ITH".
+    rewrite /smap_repr. iDestruct "SR" as "(SM & % & SR)".
+    rewrite {2 5}(map_split smap i) ITH /=.
+    rewrite !big_sepM_union.
+    2: apply map_disjoint_singleton_l_2; by apply lookup_delete.
+    iDestruct "SR" as "[S SR]". rewrite !big_sepM_singleton.
+    iFrame.
+    2: { apply map_disjoint_dom. set_solver. }
+    iIntros. iSplitR; [done| ]. iFrame.
+    iApply (big_sepM_impl with "[$]"). iIntros "!> %% %OTHER".
+    apply lookup_delete_Some in OTHER as [? ?%mk_is_Some%elem_of_dom]. 
+    rewrite /ex_ith_sig. rewrite OTHER_PRES; [by iIntros; iFrame| ..]; done. 
+  Qed.
+
+  (* TODO: use bupd in definition of OU *)
+  Lemma smap_create_ep i B K smap π π__cp τ d__h d__l
+    (PH_LE: phase_le π__cp π)
+    (LT: i < K)
+    (DEG_LT: deg_lt d__l d__h):
+    ⊢ smap_repr B K smap -∗ 
+      cp π__cp d__h (oGS := oGS) -∗
+      th_phase_ge τ π (oGS := oGS) -∗
+      |==> OU (∃ s, ith_sig i s ∗
+                    ep s π__cp d__l (oGS := oGS) ∗ smap_repr B K smap ∗
+                    th_phase_ge τ π (oGS := oGS)) (oGS := oGS).
+  Proof using DISCR__d DISCR__l LEQUIV__l.
+    iIntros "SR CP PH".
+    rewrite /smap_repr. iDestruct "SR" as "(AUTH & %DOM & SIGS)".
+    assert (i ∈ dom smap) as [s ITH]%elem_of_dom.
+    { rewrite DOM. apply elem_of_set_seq. lia. }
+    rewrite {2 5}(map_split smap i) ITH /=.
+    setoid_rewrite big_sepM_union.
+    2, 3: apply map_disjoint_singleton_l_2; by apply lookup_delete.
+    iDestruct "SIGS" as "[SIG SIGS]". setoid_rewrite big_sepM_singleton.
+    rewrite {1}/ex_ith_sig. 
+    iDestruct (create_ep_upd with "CP [$] [PH]") as "OU".
+    { eauto. }
+    { done. }
+    { done. }
+    iMod (own_update with "AUTH") as "X". 
+    { apply auth_update_dfrac_alloc. 
+      2: { apply singleton_included_l with (i := i).
+           rewrite lookup_fmap ITH. eexists. split; [| reflexivity].
+           simpl. reflexivity. }
+      apply _. }
+    iApply (OU_wand with "[-OU]"); [| by iFrame].
+    iIntros "(EP & SIG & PH)".
+    iDestruct "X" as "[? ITH]". 
+    iExists _. iFrame. done.
+  Qed.
+
+  (* TODO: move, find existing? *)
+  Lemma lookup_delete_ne' `{Countable K} {V: Type} (k: K) (m: gmap K V)
+    (NOk: k ∉ dom m):
+    delete k m = m.
+  Proof using.
+    apply map_eq. intros.
+    destruct (decide (i = k)) as [-> | ?].
+    - rewrite lookup_delete. symmetry.
+      by apply not_elem_of_dom.
+    - by apply lookup_delete_ne.
+  Qed.                          
+
+  Lemma smap_sgns_extend (B B': nat -> bool)
+    (smap: gmap nat SignalId) (s : SignalId) (m : nat) (* lm *)
+    (DOM: dom smap = set_seq 0 m)
+    (PRES: forall i, i ∈ dom smap -> B' i = B i)
+    :
+    ⊢ ([∗ map] k↦y ∈ smap, sgn y (L k) (Some (B k)) (oGS := oGS)) -∗
+       sgn s (L m) (Some (B' m)) (oGS := oGS) -∗
+       [∗ map] i↦s0 ∈ <[m := s]> smap, sgn s0 (L i) (Some $ B' i) (oGS := oGS).
+  Proof using.
+    iIntros "SIGS SG".
+    rewrite big_opM_insert_delete. 
+    iSplitL "SG"; [done| ].
+    rewrite lookup_delete_ne'.
+    2: { rewrite DOM. intros ?%elem_of_set_seq. lia. }
+    iApply (big_sepM_impl with "[$]"). iModIntro.
+    iIntros (??) "% ?".
+    rewrite PRES; [done| ].
+    eapply elem_of_dom; eauto. 
+  Qed.
+
+  Lemma BMU_smap_extend `{invGS_gen HasNoLc Σ} τ m smap R
+    (B B': nat -> bool)
+    (PRES: forall i, i ∈ dom smap -> B' i = B i)
+    (FRESH_UNSET: B' m = false):
+    ⊢ obls τ R (oGS := oGS) -∗ smap_repr B m smap -∗
+      BMU ∅ 1 (
+        |==> (∃ s',
+             smap_repr B' (m + 1) (<[m := s']> smap) ∗
+             ith_sig m s' ∗ obls τ (R ∪ {[s']}) (oGS := oGS) ∗
+             ⌜ s' ∉ R ⌝)) (oGS := oGS).
+    Proof using LEQUIV__l DISCR__l DISCR__d.
+      iIntros "OBLS SM".
+      iApply OU_BMU.
+      iDestruct (OU_create_sig with "OBLS") as "FOO".
+      iApply (OU_wand with "[-FOO]"); [| by iFrame].
+      iIntros "(%s' & SG & OBLS & %NEW)".
+      iApply BMU_intro.
+      rewrite /smap_repr. iDestruct "SM" as "(SM & %DOM & SIGS)". 
+      iMod (own_update with "SM") as "SM".
+      { apply auth_update_alloc. eapply (alloc_singleton_local_update _ m (to_agree s')).
+        2: done.
+        apply not_elem_of_dom. rewrite dom_fmap. rewrite DOM.
+        intros ?%elem_of_set_seq. lia. }
+      iModIntro. iDestruct "SM" as "[SM S']".
+      iExists s'.
+      rewrite -fmap_insert. iFrame. iSplit; [| done].
+      iSplitR.
+      { iPureIntro. rewrite dom_insert_L.
+        rewrite set_seq_add_L. rewrite -DOM. set_solver. }
+      iApply (smap_sgns_extend with "[$]"); try done.
+      rewrite FRESH_UNSET. iFrame.
+    Qed.
+      
+    Lemma ith_sig_expect i sw m τ π π__e smap R d B
+      (PH_EXP: phase_le π__e π)
+      (UNSETi: B i = false):
+      ⊢ ep sw π__e d (oGS := oGS) -∗ th_phase_ge τ π (oGS := oGS) -∗
+         smap_repr B m smap -∗ ith_sig i sw -∗
+         obls τ R (oGS := oGS) -∗ sgns_level_gt R (L i) (oGS := oGS) -∗ 
+         OU (∃ π', cp π' d (oGS := oGS) ∗ smap_repr B m smap ∗ th_phase_ge τ π' (oGS := oGS) ∗ obls τ R (oGS := oGS) ∗ ⌜ phase_le π π' /\ phase_le π__e π' ⌝) (oGS := oGS).
+    Proof using LEQUIV__l DISCR__l.
+      iIntros "#EP PH SR #SW OBLS #OBLS_LT". 
+      iDestruct (ith_sig_in with "[$] [$]") as "%ITH".
+      iDestruct (smap_repr_split with "SW [$]") as "[SGw SR]".
+      rewrite {1}/ex_ith_sig. rewrite UNSETi. 
+      iDestruct (expect_sig_upd with "EP [$] [$] [$] [$]") as "OU"; [done| ..].
+      iApply (OU_wand with "[-OU]"); [| done].
+      iIntros "(%π' & CP1 & SIGW & OBLS & PH & [%PH_LE' %PH_LE''])".
+      iExists _. iFrame. iSplitL; [| done].
+      iApply "SR". rewrite /ex_ith_sig. by rewrite UNSETi.
+    Qed.
+
+    Lemma smap_expose_dom B m smap:
+      ⊢ smap_repr B m smap -∗ ⌜ dom smap = set_seq 0 m ⌝.
+    Proof using. by iIntros "(?&?&?)". Qed.
+
+End SignalMap.
+
+
+Section SignalsBlock.
+
+  Definition sigs_block (smap: gmap nat SignalId) from len: list SignalId :=
+    map (fun k => default 0 (smap !! k)) (seq from len).
+
+  Lemma sigs_block_in smap from len:
+    forall s i, smap !! i = Some s -> i ∈ seq from len -> s ∈ sigs_block smap from len.
+  Proof using.
+    intros ?? ITH DOM. rewrite /sigs_block.
+    apply elem_of_list_In. apply in_map_iff. setoid_rewrite <- elem_of_list_In. 
+    eexists. split; eauto. by rewrite ITH.
+  Qed.
+
+  Lemma sigs_block_len smap from len: length $ sigs_block smap from len = len.
+  Proof using.
+    rewrite /sigs_block. by rewrite map_length seq_length.
+  Qed.
+
+  Lemma sigs_block_is_Some smap from len:
+    forall k, is_Some (sigs_block smap from len !! k) <-> k < len.
+  Proof using.
+    intros. 
+    rewrite lookup_lt_is_Some. by rewrite sigs_block_len.
+  Qed.
+
+  Lemma sigs_block_lookup_eq smap from len:
+    forall k, k < len -> from + k ∈ dom smap -> sigs_block smap from len !! k = smap !! (from + k). 
+  Proof using.
+    intros ? DOMsb DOMm.
+    rewrite /sigs_block.
+    rewrite list_lookup_fmap.
+    rewrite lookup_seq_lt; [| done]. simpl.
+    apply elem_of_dom in DOMm as [? DOMm]. by rewrite DOMm.
+  Qed. 
+
+End SignalsBlock.
